Fixing the bigstep proof and a few things used for the retrofitted semantics

hol/retrofit_sem/p4_exec_wrapper_ffiLib.sig
@@ -2,6 +2,6 @@ signature p4_exec_wrapper_ffiLib =
 sig
   include Abbrev
 
-val translate_p4 : string -> term -> term -> term -> term -> bool -> bool -> unit
+val translate_p4 : string -> term -> term -> term -> bool -> bool -> unit
 
 end
